veric/NullExtension.v
@@ -19,7 +19,7 @@ Definition dryspec : external_specification juicy_mem external_function unit
      (fun rv m z => False).
 
 Definition Espec : OracleKind.
- refine (Build_OracleKind unit (Build_juicy_ext_spec _ dryspec _ _ _)).
+ refine (Build_OracleKind (ghost_PCM.discrete_PCM unit) (Build_juicy_ext_spec _ dryspec _ _ _)).
 Proof.
 simpl; intros; contradiction.
 simpl; intros; contradiction.
